theories/SystemF/Reductions/HaltTM_1_to_SysF_TYP.v
@@ -2,24 +2,27 @@
   Reduction from:
     Turing Machine Halting (HaltTM 1)
   to:
-    Semi-unification (SemiU)
+    System F Typability (SysF_TYP)
 *)
 
 Require Import Undecidability.Synthetic.Definitions Undecidability.Synthetic.ReducibilityFacts.
 
 Require Import Undecidability.TM.TM.
-Require Import Undecidability.SemiUnification.SemiU.
+Require Import Undecidability.SystemF.SysF.
 
 Require Undecidability.StackMachines.Reductions.HaltTM_1_to_CSSM_UB.
 Require Undecidability.SemiUnification.Reductions.CSSM_UB_to_SSemiU.
 Require Undecidability.SemiUnification.Reductions.SSemiU_to_RU2SemiU.
-Require Undecidability.SemiUnification.Reductions.RU2SemiU_to_SemiU.
+Require Undecidability.SemiUnification.Reductions.RU2SemiU_to_LU2SemiU.
 
-(** Many-one reduction from Turing machine halting to semi-unification *)
-Theorem reduction : HaltTM 1 ⪯ SemiU.
+Require Undecidability.SystemF.Reductions.LU2SemiU_to_SysF_TYP.
+
+(** Many-one reduction from Turing machine halting to System F typability*)
+Theorem reduction : HaltTM 1 ⪯ SysF_TYP.
 Proof.
   apply (reduces_transitive HaltTM_1_to_CSSM_UB.reduction).
   apply (reduces_transitive CSSM_UB_to_SSemiU.reduction).
   apply (reduces_transitive SSemiU_to_RU2SemiU.reduction).
-  exact RU2SemiU_to_SemiU.reduction.
+  apply (reduces_transitive RU2SemiU_to_LU2SemiU.reduction).
+  exact LU2SemiU_to_SysF_TYP.reduction.
 Qed.
